working on codegen

Scratch.thy
@@ -1,41 +1,21 @@
 theory "Scratch"
 imports Main  "./Proof_Checker"
 begin
-  
-
-
 type_synonym arity = Enum.finite_5
 
-
+(*code_thms dl.Proof_Checker.proof_result dl.Proof_Checker.proof_ok*)
+(*print_codesetup*)
+(*export_code dl.Proof_Checker.proof_ok dl.Proof_Checker.proof_result in SML*)
+(*module_name Example file "examples/"**)
+  
 datatype myvars =
     i1
   | i2
   | i3
   | i4
   | i5
-
-    
-instantiation myvars :: enum begin
-definition "enum_myvars == [i1, i2, i3, i4, i5]"
-definition "enum_all_myvars = (\<lambda>f. f i1 \<and> f i2 \<and> f i3 \<and> f i4 \<and> f i5)"
-definition "enum_ex_myvars = (\<lambda>f. f i1 \<or> f i2 \<or> f i3 \<or> f i4 \<or> f i5)"
-instance 
-  apply(standard)
-  subgoal 
-    apply(auto simp add: enum_myvars_def)
-    using myvars.exhaust enum_myvars_def by blast
-  subgoal
-    by(auto simp add: enum_myvars_def) 
-  subgoal for P
-    apply(unfold enum_all_myvars_def)
-    by (metis UNIV_I myvars.exhaust)
-  subgoal for P
-    apply(unfold enum_ex_myvars_def)
-    by (metis UNIV_I myvars.exhaust)
-  done      
-end
   
-(*instantiation myvars :: finite begin
+instantiation myvars :: finite begin
 instance proof
   have "UNIV = {i1, i2, i3, i4, i5}"
     unfolding UNIV_def 
@@ -47,8 +27,36 @@ instance proof
     by auto
 qed
 end
-  *)
     
+  (*   fixes enum :: "'a list"
+  fixes enum_all :: "('a \<Rightarrow> bool) \<Rightarrow> bool"
+  fixes enum_ex :: "('a \<Rightarrow> bool) \<Rightarrow> bool"
+  assumes UNIV_enum: "UNIV = set enum"
+    and enum_distinct: "distinct enum"
+  assumes enum_all_UNIV: "enum_all P \<longleftrightarrow> Ball UNIV P"
+  assumes enum_ex_UNIV: "enum_ex P \<longleftrightarrow> Bex UNIV P" *)
+instantiation myvars :: enum begin
+definition enum_myvars where   "enum_myvars \<equiv> [i1, i2, i3, i4, i5]"
+definition enum_all_myvars where "enum_all_myvars P \<equiv> list_all P [i1, i2, i3, i4, i5]"
+definition enum_ex_myvars where "enum_ex_myvars P \<equiv> list_ex P [i1, i2, i3, i4, i5]"
+instance
+  apply(standard)
+  subgoal apply auto
+    subgoal for x
+      by(cases x, auto simp add: enum_myvars_def)
+    done
+    apply (auto simp add: enum_myvars_def)
+  subgoal for P x
+    by(cases x, auto simp add: enum_myvars_def enum_all_myvars_def)
+  subgoal for P
+    by(auto simp add: enum_myvars_def enum_all_myvars_def)
+  subgoal for P
+    by(auto simp add: enum_myvars_def enum_ex_myvars_def)
+  subgoal for P x
+    by(cases x, auto simp add: enum_myvars_def enum_ex_myvars_def)
+  done
+end
+  
 instantiation myvars :: linorder begin
 definition less_eq_myvars where
   "x \<le> y \<equiv> 
@@ -97,166 +105,19 @@ definition x::myvars where "x = i1"
 definition y::myvars where "y = i2"
 definition z::myvars where "z = i3"
 definition w::myvars where "w = i4"
-
-
   
-global_interpretation ddl : ids x y z x y z x y z w
-  defines proof_result   = ddl.proof_result
-    and   rrule_ok       = ddl.rrule_ok
-    and   lrule_ok       = ddl.lrule_ok
-    and   step_ok        = ddl.step_ok
-    and   deriv_ok       = ddl.deriv_ok
-    and   proof_ok       = ddl.proof_ok
-    and   start_proof    = ddl.start_proof
-    and   deriv_result   = ddl.deriv_result
-    and   step_result    = ddl.step_result
-    and   get_axiom      = ddl.get_axiom
-    and   Rrule_result   = ddl.Rrule_result
-    and   Lrule_result   = ddl.Lrule_result
-    and   ssafe          = ddl.ssafe
-    and   Padmit_Fadmit  = ddl.Padmit_Fadmit
-    and   Padmit         = ddl.Padmit
-    and   Fadmit         = ddl.Fadmit
-    and   diff_times_axiom = ddl.diff_times_axiom
-    and   diff_const_axiom = ddl.diff_const_axiom
-    and   diff_plus_axiom = ddl.diff_plus_axiom
-    and   DIGeqaxiom = ddl.DIGeqaxiom
-    and   DIGraxiom = ddl.DIGraxiom
-    and   DWaxiom = ddl.DWaxiom
-    and   DSaxiom = ddl.DSaxiom
-    and   DGaxiom = ddl.DGaxiom
-    and   DEaxiom = ddl.DEaxiom
-    and   DCaxiom = ddl.DCaxiom
-    and   loop_iterate_axiom = ddl.loop_iterate_axiom
-    and   diff_assign_axiom = ddl.diff_assign_axiom
-    and   choice_axiom = ddl.choice_axiom
-    and   assign_axiom = ddl.assign_axiom
-    and   test_axiom = ddl.test_axiom
-    and   box_axiom = ddl.box_axiom
-    and   Vaxiom = ddl.Vaxiom
-    and   Kaxiom = ddl.Kaxiom
-    and   Iaxiom = ddl.Iaxiom
-    and   state_fun = ddl.state_fun
-    and   singleton = ddl.singleton
-    and   p1 = ddl.p1
-    and   f1 = ddl.f1
-    and   f0 = ddl.f0
-    and   P = ddl.P
+global_interpretation ddl:ids x y z x y z x y z w 
+  defines ddl_proof_result = "ddl.proof_result"
+  and ddl_deriv_result = "ddl.deriv_result"
+  and ddl_start_proof = "ddl.start_proof"
+  and ddl_step_result = "ddl.step_result"
+  and ddl_Rrule_result = "ddl.Rrule_result"
+  and ddl_Lrule_result = "ddl.Lrule_result"
   by(standard, auto simp add: x_def y_def z_def w_def)
-
-declare ddl.deriv_ok.intros [code_pred_intro]
-declare ddl.proof_ok.intros [code_pred_intro]
-declare ddl.Padmit_Fadmit.intros [code_pred_intro]
-(*declare ddl.step_ok.intros [code_pred_intro]*)
-declare ddl.step_ok.Step_Axiom [code_pred_intro]
-declare ddl.step_ok.Step_AxSubst [code_pred_intro]
-declare ddl.step_ok.Step_Cut [code_pred_intro]
-declare ddl.step_ok.Step_CloseId [code_pred_intro]
-declare ddl.Step_G_code[code_pred_intro]
-declare ddl.step_ok.Step_DEAxiom_schema [code_pred_intro]
-declare ddl.step_ok.Step_Lrule[code_pred_intro]
-declare ddl.Lrule_And_code[code_pred_intro]
-declare ddl.Lrule_Imply_code[code_pred_intro]
-declare ddl.Lrule_EquivForward_code[code_pred_intro]
-declare ddl.Lrule_EquivBackward_code[code_pred_intro]
-declare ddl.step_ok.Step_Rrule[code_pred_intro]
-declare ddl.Rrule_And_code[code_pred_intro]
-declare ddl.Rrule_Imply_code[code_pred_intro]
-declare ddl.Rrule_Equiv_code[code_pred_intro]
-declare ddl.Rrule_Cohide_code[code_pred_intro]
-declare ddl.Rrule_CohideRR_code[code_pred_intro]
-declare ddl.Rrule_True[code_pred_intro]
-
-
-(*declare ddl.step_ok.Step_Rrule[code_pred_intro]*)
-
-code_pred 
-  (modes: i \<Rightarrow> i \<Rightarrow> i \<Rightarrow> i \<Rightarrow> i \<Rightarrow> bool as is_rrule_ok)
-  rrule_ok
-  sorry
-
-code_pred 
-  (modes: i \<Rightarrow> i \<Rightarrow> i \<Rightarrow> bool as is_step_ok)
-  step_ok
-  sorry
-
-code_pred 
-  (modes: i  \<Rightarrow> bool as is_proof_ok)
-  proof_ok
-  sorry
-(*declare ddl.step_ok.Step_G [code_pred_intro]*)
-
-  
-(*  Step_Axiom:"(nth SG i) = ([], [get_axiom a]) \<Longrightarrow> step_ok (SG,C) i (Axiom a)"
-| Step_AxSubst:"(nth SG i) = ([], [Fsubst (get_axiom a) \<sigma>]) \<Longrightarrow> Fadmit \<sigma> (get_axiom a) \<Longrightarrow> ssafe \<sigma> \<Longrightarrow> step_ok (SG,C) i (AxSubst a \<sigma>)"
-| Step_Lrule:"lrule_ok SG C i j L \<Longrightarrow> j < length (fst (nth SG i)) \<Longrightarrow> step_ok (SG,C) i (Lrule L j)"
-| Step_Rrule:"rrule_ok SG C i j L \<Longrightarrow> j < length (snd (nth SG i)) \<Longrightarrow> step_ok (SG,C) i (Rrule L j)"
-| Step_Cut:"fsafe \<phi> \<Longrightarrow> i < length SG \<Longrightarrow> step_ok (SG,C) i (Cut \<phi>)"
-| Step_CloseId:"nth (fst (nth SG i)) j = nth (snd (nth SG i)) k \<Longrightarrow> j < length (fst (nth SG i)) \<Longrightarrow> k < length (snd (nth SG i)) \<Longrightarrow> step_ok (SG,C) i (CloseId j k) "
-| Step_G:"\<And>a p. nth SG i = ([], [([[a]]p)]) \<Longrightarrow> step_ok (SG,C) i G"
-| Step_DEAxiom_schema:*)
-
-export_code is_proof_ok proof_result in Scala
-
-
-
-    
-export_code "step_ok.equation" in Scala
-
-code_pred deriv_ok 
-   apply(auto simp add: ddl.deriv_ok.cases)
-   apply (metis ddl.deriv_ok.cases fst_conv)
-    sorry
-(*   apply (meson ddl.step_ok.cases fst_conv insert_disjoint(2) snd_conv)*)*
-
-export_code "deriv_ok" in Scala
-
-code_pred proof_ok 
-  sorry
-    sorry
-
-(*  apply(auto)
-  subgoal
-    by (simp add: ddl.proof_ok_simps)
-  subgoal
-    by (metis ddl.deriv_ok.cases fst_conv)
-(*  apply(auto simp add: ddl.step_ok.cases fst_conv insert_disjoint(2) snd_conv)*)
-    sorry
-    *)
-             
-(*definition deriv_result::"((myvars, myvars, myvars) formula list \<times> (myvars, myvars, myvars) formula list) list \<times>
-  (myvars, myvars, myvars) formula list \<times> (myvars, myvars, myvars) formula list
-  \<Rightarrow> (nat \<times> (myvars, myvars, myvars) ddl.step) list
-     \<Rightarrow> ((myvars, myvars, myvars) formula list \<times> (myvars, myvars, myvars) formula list) list \<times>
-        (myvars, myvars, myvars) formula list \<times> (myvars, myvars, myvars) formula list"
-where "deriv_result = ids.deriv_result"
-
-*)
-(*lemmas [code] = ddl.deriv_result.simps[folded  proof_result_def]
-lemmas [code] = ddl.proof_result.simps[folded deriv_result_def proof_result_def]
-lemmas [code] = deriv_result_def[symmetric]*)
-
-(*lemmas [code] = ddl.proof_result.simps[folded proof_result_def]
-lemmas [code] = proof_result_def[symmetric]*)
-lemmas [code] = enum_all_myvars_def enum_ex_myvars_def enum_myvars_def  
-  
-code_pred "proof_ok"
-
-(*code_pred "ddl.proof_ok"*)
-export_code "proof_result"  "proof_ok" in SML
-
-definition test 
-where "test = ddl.get_axiom"
-(*code_thms "ids.get_axioms"*)
-(*print_codesetup*)
-(*export_code dl.Proof_Checker.proof_ok dl.Proof_Checker.proof_result in SML*)
-(*module_name Example file "examples/"**)
-  
-(*print_codesetup*)
-(*=export_code "ids.Tsubst" in SM*)
-export_code "ddl.Tsubst" in SML
-
 (* defines Tsubst = ddl.Tsubst*)
+
+declare ddl.proof_result.simps[code_pred_simp]  ddl.deriv_result.simps[code_pred_simp] ddl.start_proof.simps[code_pred_simp] ddl.step_result.simps[code_pred_simp]
+export_code "ddl_proof_result" in Scala
 
 (*definition foo::real where "foo = 1.234"
 export_code foo in SML*)
